4 

KABALAN GASPARD 

a k is defined to be a (k mod p) for all k /∈{0, ..., p − 1} (a p−1 = 0, trivially). And so p−2 p−2 � (a p−k − a 1 )ζ <sup>[k]</sup> = u = ζ <sup>[−][t]</sup> u = � (a k+t − a (p−1)+t )ζ <sup>[k]</sup> by 1 and therefore, since this rep- k=0 k=0 

resentation is unique, we get 

**==> formula intentionally omitted <==**

Letting k 0 be the mod p solution to k + t ≡ p − k (p), we get a k 0 +t = a p−k 0 and so (1.1) yields a (p−1)+t = a 1 . (1.1) then becomes 

**==> formula intentionally omitted <==**

Since replacing k by −(k + t) in (1.2) leaves the equation invariant, we get <sup>[p][−]</sup> 2 <sup>[1]</sup> pairs of equal terms with distinct indices amongst a 0 , ..., a p−1 (the ’remaining’ term being a k 0 +t ). Let b 1 , ..., b p−1 be representatives of these distinct pairs, and let b k 0 +t = a k 0 +t (we have simply 2 selected and reordered the a i ’s). 

Now by the proof of 1, there is a unique c modulo p such that ζ <sup>[c]</sup> u is primary, and this c p−2 is the solution to ax ≡ b (p) where u ≡ a + bλ (λ <sup>[2]</sup> ) where λ = (1 − ζ). Now u = � a k ζ <sup>[k]</sup> . k=0 

p−2 Writing, as a polynomial, f (x) = � a k x <sup>[k]</sup> , we can find a and b by finding the coefficients of k=0 1 and x respectively of f (1 − x) since ζ = 1 − λ. Making elementary use of the Binomial p−2 p−2 p−2 Theorem, we see that f (1 − x) = � a k (1 − x) <sup>[k]</sup> = � a k − � ka k x + ... (we only need the k=0 k=0 k=0 first two terms). So c is the solution to 

p−2 

**==> formula intentionally omitted <==**

Which, since a p−1 = 0, is equivalent to 

p−1 

**==> formula intentionally omitted <==**

Now k 0 + t ≡ p − k 0 (p) ⇒ k 0 + t ≡−(k 0 + t) + t (p) ⇒ (k 0 + t) ≡ 2 <sup>[−][1]</sup> t ⇒ b k 0 +t = a k 0 +t = a 2 −1 t . Finally, note that for a i = a t−i = b l for 1 ≤ l ≤ <sup>[p][−]</sup> 2 <sup>[1]</sup> by (1.2), ia i + (t − i)a t−i = tb l . 

