4

KABALAN GASPARD

ak is defined to be a(k modp) for all k ‡ {0,...,p 1} (ap-1 - = 0, trivially). And so
p-2 p-2
Σ(ap-k - α1) = u = 5-tu u = Σ (ak+ta (p-1)+t) ( by 1 and therefore, since this rep-
k=0 k=0
resentation is unique, we get

(1.1) ak+t - a(p-1)+t = ap-k a₁ for all 0 ≤ k ≤ p − 1 -

Letting k0 be the mod p solution to k + t ≡ p − k (p), we get ak0+t = a p−k0 and so (1.1) yields a( p−1)+t = a1. (1.1) then becomes

(1.2) ak+t = ap-k = a_k for all 0 ≤ k ≤ p − 1

Since replacing k by −(k + t) in (1.2) leaves the equation invariant, we get P21 pairs of equal terms with distinct indices amongst ao, ..., ap-1 (the 'remaining' term being ako+t). Let b₁,, bp be representatives of these distinct pairs, and let bko+t =ako+t (we have simply selected and reordered the a;'s).

Now by the proof of 1, there is a unique c modulo p such that ζ c u is primary, and this c p-2 is the solution to ax = b (p) where u = a + bλ (x²) where > = (1). Now u = Σακς. k=0 p-2 Writing, as a polynomial, f(x) = Σaxk, we can find a and b by finding the coefficients of k=0 1 and x respectively of f(1 - x) since ( = 1 - A. Making elementary use of the Binomial p-2 Theorem, we see that f(1 - x) = Σ ak(1 − x)k = Σ ak − Σ kakx + ... (1-x)=ak-k (we only need the k=0 k=0 k=0 first two terms). So c is the solution to

p-2
(1.3) (E) == E x Σ kak (p)
k=0 k=0

Which, since ap-1 = 0, is equivalent to

p-1 p-1
(1.4) (Em) ==-Am (10) ак kak
k=0 k=0

Now kot = p − ko (p) ⇒ ko+t= −(ko+t) +t (p) ⇒ (ko+t) = 2¯¹t ⇒ bko+t : = ako+t = a2-1. Finally, note that for a¿ = at−i = bɩ for 1 ≤1 ≤ º±¹ by (1.2), iar + (t − i)at−i = tbɩ. -