4 

KABALAN GASPARD 

ak is defined to be a(k mod p) for all k /∈{0, ..., p − 1} (ap−1 = 0, trivially). And so p−2 p−2 � (ap−k − a1)ζ[k] = u = ζ[−][t] u = � (ak+t − a(p−1)+t)ζ[k] by 1 and therefore, since this repk=0 k=0 resentation is unique, we get 

**==> formula [357 x 21] intentionally omitted <==**

Letting k0 be the mod p solution to k + t ≡ p − k (p), we get ak0+t = ap−k0 and so (1.1) yields a(p−1)+t = a1. (1.1) then becomes 

**==> formula [335 x 21] intentionally omitted <==**

Since replacing k by −(k + t) in (1.2) leaves the equation invariant, we get[p][−] 2[1] pairs of equal terms with distinct indices amongst a0, ..., ap−1 (the ’remaining’ term being ak0+t). Let b1, ..., b p−1 be representatives of these distinct pairs, and let bk0+t = ak0+t (we have simply 2 selected and reordered the ai’s). 

Now by the proof of 1, there is a unique c modulo p such that ζ[c] u is primary, and this c p−2 is the solution to ax ≡ b (p) where u ≡ a + bλ (λ[2] ) where λ = (1 − ζ). Now u = � akζ[k] . k=0 

p−2 Writing, as a polynomial, f (x) = � akx[k] , we can find a and b by finding the coefficients of k=0 1 and x respectively of f (1 − x) since ζ = 1 − λ. Making elementary use of the Binomial p−2 p−2 p−2 Theorem, we see that f (1 − x) = � ak(1 − x)[k] = � ak − � kakx + ... (we only need the k=0 k=0 k=0 first two terms). So c is the solution to 

p−2 

**==> formula [306 x 39] intentionally omitted <==**

Which, since ap−1 = 0, is equivalent to 

p−1 

**==> formula [306 x 38] intentionally omitted <==**

Now k0 + t ≡ p − k0 (p) ⇒ k0 + t ≡−(k0 + t) + t (p) ⇒ (k0 + t) ≡ 2[−][1] t ⇒ bk0+t = ak0+t = a2−1t. Finally, note that for ai = at−i = bl for 1 ≤ l ≤[p][−] 2[1] by (1.2), iai + (t − i)at−i = tbl. 

