
in (a) and (b), respectively. Therefore, from consideration of Case a, b and c,

$$\sup_{\{B_k\}_{k=-\infty}^{\infty}} \sum_{k=-\infty}^{\infty} \max \{\mu_{0,W} (B_k|w) - \mu_{1,W} (B_k^D|w) , 0\}$$

$$= \sup_{\{b_k\}_{k=-\infty}^{\infty}} \sum_{k=-\infty}^{\infty} \max \left\{ F_{0,W} (b_k|w) - F_{1,W} \left( \frac{t_1 - t_W}{t_0 - t_W} b_{k+1} - \frac{t_1 - t_0}{t_0 - t_W} w|w \right) , 0 \right\}$$

where $\frac{t_0-t_W}{t_1-t_0} \delta + w \leq b_{k+1} \leq b_k$. Consequently, the sharp upper bound is written as follows: letting $F_{\Delta,W}^U (\delta|w)$ be the sharp upper bound on $\Pr (Y_1 - Y_0 \leq \delta|W = w)$ ,

$$F_{\Delta}^U (\delta)$$

$$= \int F_{\Delta,W}^U (\delta|w) dF_W (w)$$

$$= \int \left\{ 1 - \sup_{\{B_k\}_{k=-\infty}^{\infty}} \sum_{k=-\infty}^{\infty} \max \{\mu_{0,W} (B_k|w) - \mu_{1,W} (B_k^D|w) , 0\} \right\} dF_W$$

$$= 1 + \int \inf_{\{b_k\}_{k=-\infty}^{\infty}} \sum_{k=-\infty}^{\infty} \min \left\{ F_{1,W} \left( \frac{t_1 - t_W}{t_0 - t_W} b_{k+1} - \frac{t_1 - t_0}{t_0 - t_W} w|w \right) - F_{0,W} (b_k|w) , 0 \right\} dF_W$$

where $\frac{t_0-t_W}{t_1-t_0} \delta + w \leq b_{k+1} \leq b_k$. â– 

## Appendix B

Appendix B presents the procedure used to compute the sharp lower bound under MTR in Section 4 and Section 5. The following lemma is useful for reducing computational costs:

### Lemma B.1 
Let

$$\{a_k\}_{k=-\infty}^{\infty} \in \arg \max_{\{a_k\}_{k=-\infty}^{\infty} \in A_\delta} \sum_{k=-\infty}^{\infty} \max \{F_1 (a_{k+1}) - F_0 (a_k) , 0\} ,$$

where $A_\delta = \{\{a_k\}_{k=-\infty}^{\infty} : 0 \leq a_{k+1} - a_k \leq \delta \text{ for each integer } k\}$ .

It is innocuous to assume that $\{a_k\}_{k=-\infty}^{\infty}$ satisfies $a_{k+2} - a_k > \delta$ for each integer $k$.

**Proof.** I will show that for any sequence $\{a_k\}_{k=-\infty}^{\infty} \in A_\delta$ satisfying $a_{k+2} - a_k \leq \delta$ for some integer $k$, one can construct $\{\tilde{a}_k\}_{k=-\infty}^{\infty} \in A_\delta$ with $\tilde{a}_{k+2} - \tilde{a}_k > \delta$ for each integer $k$ and

$$\sum_{k=-\infty}^{\infty} \max \{F_1 (a_{k+1}) - F_0 (a_k) , 0\} \leq \sum_{k=-\infty}^{\infty} \max \{F_1 (\tilde{a}_{k+1}) - F_1 (\tilde{a}_k) , 0\} .$$

72
